src/Parsers/exampleArithmetic.dfy
@@ -2,12 +2,41 @@ include "parser.dfy"
 
 module ArithmeticParser {
   import opened StringParsers
-  import opened Printer
+  import opened StringNat
+
+  type Result<A, B> = StringParsers.Wrappers.Result<A, B>
 
   datatype Expression =
     | Binary(op: string, left: Expression, right: Expression)
-    | Number(x: int)
+    | Number(value: int)
+    | Unknown(power: int)
   {
+    function Distribute(): Result<Expression, string> {
+      match this {
+        case Number(x: int) => Result.Success(this)
+        case Binary(op, left, right) =>
+          var l :- left.Distribute();
+          var r :- right.Distribute();
+          if l.Number? && r.Number? then
+            match op {
+              case "+" => Result.Success(Number(l.value + r.value))
+              case "-" => Result.Success(Number(l.value - r.value))
+              case "*" => Result.Success(Number(l.value * r.value))
+              case "/" => 
+                if r.value == 0 then Result.Failure("Division by zero (" + right.ToString(0) + " evaluates to zero)") else
+                Result.Success(Number(l.value / r.value))
+              case "%" =>
+                if r.value == 0 then Result.Failure("Modulo by zero (" + right.ToString(0) + " evaluates to zero)") else
+                Result.Success(Number(l.value % r.value))
+              case _ => Result.Failure("Unsupported operator: " + op)
+            }
+         else
+           Result.Success(this)
+        case Unknown(0) => Result.Success(Number(1))
+        case Unknown(_) =>
+          Result.Success(this)
+      }
+    }
     static function BinaryBuilder(op: string): (Expression, Expression) -> Expression
     {
       (left: Expression, right: Expression) => Binary(op, left, right)
@@ -20,11 +49,15 @@ module ArithmeticParser {
       requires level <= 2
     {
       match this
-      case Number(x) => (if x < 0 then "-" else "") + Printer.natToString(if x < 0 then -x else x)
+      case Number(x) => (if x < 0 then "-" else "") + StringNat.natToString(if x < 0 then -x else x)
       case Binary(op, left, right) => 
         (match level case 0 => "(" case 1 => "[" case 2 => "{")
-        + left.ToString((level + 1)%3) + op + right.ToString((level + 1) % 3)
+        + left.ToString(level) + op + right.ToString(level)
         + (match level case 0 => ")" case 1 => "]" case 2 => "}")
+      case Unknown(power) =>
+        if power == 1 then "x" else if power == 0 then "1" else
+        if power < 0 then "x^(-" + StringNat.natToString(0-power)+")" else
+        "x^" + StringNat.natToString(power)
     }
   }
 
@@ -34,35 +67,44 @@ module ArithmeticParser {
      Binary(result.1.value.0, result.0, result.1.value.1))
 
   const parser: Parser<Expression>
-    := FixpointMap(
+    := ConcatL(
+      FixpointMap(
       map[
         "atom" :=
           RecursiveDef(0, (callback: ParserSelector<Expression>) => 
           Or(ConcatR(
-              Const?("("),
-                ConcatL(callback("term"), Const(")"))),
-             Map(Int(), (result: int) => Number(result))    
-            )),
+            String("("), ConcatL(
+            callback("term"),
+            String(")"))),
+          Or(
+            Map(Int(), (result: int) => Number(result)), ConcatR(
+            String("x"),
+              Map(Maybe(ConcatR(
+                String("^"), Int())),
+                  (result: Option<int>) =>
+                    if result.Some? then Unknown(result.value) else Unknown(1)
+          ))))),
         "factor" :=
           RecursiveDef(1, (callback: ParserSelector<Expression>) => 
-            Map(
-            Concat(
-              callback("atom"),
-              Maybe(Concat(Or(Const?("*"), Const?("/")),
-                     callback("factor")))),
-            buildParsedExpr
-          )),
+            Bind(callback("atom"), (atom: Expression) =>
+              RepeatAcc(
+                Concat(Or(String("*"), Or(String("/"), String("%"))),
+                   callback("atom")),
+                Expression.InfixBuilder(), atom)
+              )
+          ),
         "term" :=
           RecursiveDef(2, (callback: ParserSelector<Expression>) => 
-            Map(
-            Concat(callback("factor"),
-            Maybe(Concat(Or(Const?("+"), Const?("-")),
-                   callback("term")))),
-            buildParsedExpr
-          ))
+            Bind(callback("factor"), (factor: Expression) =>
+              RepeatAcc(
+                Concat(Or(String("+"), String("-")),
+                   callback("factor")),
+                Expression.InfixBuilder(), factor)
+              )
+          )
       ],
       "term"
-    );
+    ), EndOfString())
 
   method Main(args: seq<string>) {
     if |args| <= 1 {
@@ -70,12 +112,19 @@ module ArithmeticParser {
     }
     for i := 1 to |args| {
       var input := args[i];
-      Succeed_NonCrashingAuto<Expression>();
-      assume {:axiom} Valid(parser); // TODO: Prove
-      reveal Valid();
       match parser(input) {
-        case PSuccess(result, _) =>
-          print "result:", result.ToString(0), "\n";
+        case PSuccess(result, remaining) =>
+          if |remaining| != 0 {
+            print "'" + remaining +"'", "\n";
+            PrintFailure<int>(input, PFailure(Recoverable, FailureData("Expected end of string", remaining, Option.None)));
+          }
+          print "Computation:", result.ToString(0), "\n";
+          match result.Distribute() {
+            case Success(x) =>
+              print "Result:", x.ToString(0), "\n";
+            case Failure(message) =>
+              print message;
+          }
         case failure =>
           PrintFailure(input, failure);
       }
